[kemedhoc][low-star] Msg2 Responder's side, high-level API done

src/kemedhoc/Impl.KEMEDHOC.Core.Msg2.Aux.fst
@@ -40,6 +40,7 @@ open Impl.KEMEDHOC.Parser
 open Impl.KEMEDHOC.Ciphertext
 open Impl.KEMEDHOC.TranscriptHash
 open Impl.KEMEDHOC.Core
+open Impl.KEMEDHOC.Core.Utilities
 open Spec.KEMEDHOC.Base.Definitions
 
 (*-------------- Utilities*)
@@ -207,6 +208,9 @@ val initiator_process_msg2_set_up:
     /\ is_valid_handshake_state_m h1 hs
     /\ is_valid_party_state_m h1 is
     /\ is_valid_message2 h1 msg2
+
+    /\ lbufferOpt_is_Some h1 hs.k_xy /\ lbufferOpt_is_Some h1 hs.k_auth_I
+    /\ lbufferOpt_is_Some h1 hs.th2 /\ lbufferOpt_is_Some h1 hs.prk2e
   )
 
 #push-options "--z3rlimit 30 --max_fuel 4 --max_ifuel 4"
@@ -244,32 +248,180 @@ let initiator_process_msg2_set_up kcs is hs msg2
 
 #pop-options
 
+#push-options "--z3rlimit 40"
+let initiator_process_msg2_decrypt_c2_uti (#kcs: supportedKemCipherSuite)
+  (hs: handshake_state_m kcs) (is: party_state_m kcs)
+  (ptx2: plaintext2 kcs)
+  : ST.Stack c_response
+  (requires fun h0 ->
+    is_valid_handshake_state_m h0 hs
+    /\ is_valid_party_state_m h0 is
+    /\ is_valid_plaintext2 h0 ptx2
 
-// val initiator_process_msg2_decrypt_c2:
-//   kcs: supportedKemCipherSuite
-//   -> is: party_state_m kcs
-//   -> hs: handshake_state_m kcs
-//   -> msg2: message2 kcs
-//   -> ptx2: plaintext2 kcs
-//   -> ST.Stack c_response
-//   (requires fun h0 ->
-//     is_valid_handshake_state_m h0 hs /\ is_valid_handshake_state_init h0 hs
-//     /\ is_valid_party_state_m h0 is
-//     /\ is_valid_message2 h0 msg2
-//     /\ is_valid_plaintext2 h0 ptx2
+    // Disjointness
+    /\ handshake_state_m_disjoint_to_party_state hs is
+    /\ handshake_state_m_disjoint_to_p2 hs ptx2
+    /\ party_state_disjoint_to_p2 is ptx2
+  )
+  (ensures fun h0 res h1 ->
+    modifies0 h0 h1
+    /\ (match res with
+        | TypeEdhoc.CInvalidCredential
+        | TypeEdhoc.CIntegrityCheckFailed
+        | TypeEdhoc.CSuccess -> True
+        | _ -> False
+    )
+  )
+  = ST.push_frame();
+  (**) let h0 = ST.get () in
 
-//     // Disjointness
-//     /\ handshake_state_m_disjoint_to_party_state hs is
-//     /\ handshake_state_m_disjoint_to_msg2 hs msg2
-//     /\ handshake_state_m_disjoint_to_p2 hs ptx2
-//     /\ party_state_disjoint_to_msg2 is msg2
-//     /\ party_state_disjoint_to_p2 is ptx2
-//     /\ message2_disjoint_to_p2 msg2 ptx2
-//   )
-//   (ensures fun h0 res h1 ->
-//     True
-//   )
+  // check credential ID
+  let res = check_credential ptx2.id_cred_R is.remote_id_cred in
+  let final_res = match res with
+    | TypeEdhoc.CInvalidCredential -> res
+    | TypeEdhoc.CSuccess -> (
+      // construct context2
+      let ctx2: context2 kcs = {
+        c_r = ptx2.c_R;
+        id_cred_r = ptx2.id_cred_R;
+        th2 = hs.th2.value;
+        cred_r = ptx2.cred_R;
+      } in
 
+      // derive MAC2
+      let mac2 = create (size (SpecCrypto.mac23_size kcs)) (u8 0) in
+      expand_mac2 #kcs hs.prk3e2m.value ctx2 mac2;
+      (**) let h2 = ST.get () in
+
+      // check MAC2
+      check_mac #kcs mac2 ptx2.mac2
+
+    ) in
+
+  ST.pop_frame();
+  final_res
+
+#pop-options
+
+val initiator_process_msg2_decrypt_c2:
+  kcs: supportedKemCipherSuite
+  -> is: party_state_m kcs
+  -> hs: handshake_state_m kcs
+  -> msg2: message2 kcs
+  -> ptx2: plaintext2 kcs
+  -> ST.Stack c_response
+  (requires fun h0 ->
+    is_valid_handshake_state_m h0 hs
+    /\ is_valid_party_state_m h0 is
+    /\ is_valid_message2 h0 msg2
+    /\ is_valid_plaintext2 h0 ptx2
+
+    /\ lbufferOpt_is_Some h0 hs.th2 /\ lbufferOpt_is_Some h0 hs.prk2e
+    /\ lbufferOpt_is_Some h0 hs.k_auth_I /\ lbufferOpt_is_Some h0 hs.k_xy
+
+    // Disjointness
+    /\ handshake_state_m_disjoint_to_party_state hs is
+    /\ handshake_state_m_disjoint_to_msg2 hs msg2
+    /\ handshake_state_m_disjoint_to_p2 hs ptx2
+    /\ party_state_disjoint_to_msg2 is msg2
+    /\ party_state_disjoint_to_p2 is ptx2
+    /\ message2_disjoint_to_p2 msg2 ptx2
+  )
+  (ensures fun h0 res h1 ->
+    let modified_locs = lbufferOpt_loc hs.prk3e2m
+                          |+| plaintext2_union ptx2 in
+    (match res with
+      | TypeEdhoc.CUnsupportedAlgorithmOrInvalidConfig
+      | TypeEdhoc.CDecryptionFailure -> modifies0 h0 h1
+      | TypeEdhoc.CInvalidCredential
+      | TypeEdhoc.CIntegrityCheckFailed
+      | TypeEdhoc.CSuccess -> (
+        modifies modified_locs h0 h1
+        /\ lbufferOpt_is_Some h1 hs.prk3e2m
+      )
+      | _ -> False  
+    )
+    /\ is_valid_handshake_state_m h1 hs
+    /\ is_valid_party_state_m h1 is
+    /\ is_valid_message2 h1 msg2
+  )
+
+#push-options "--z3refresh --z3rlimit 60 --max_fuel 2 --max_ifuel 2"
+let initiator_process_msg2_decrypt_c2_set_up (#kcs: supportedKemCipherSuite)
+  (hs: handshake_state_m kcs) (p2: plaintext2 kcs)
+  (ptx2_buffer: plaintext2_buff kcs)
+  : ST.Stack unit
+  (requires fun h0 ->
+    is_valid_handshake_state_m h0 hs
+    /\ is_valid_plaintext2 h0 p2
+    /\ live h0 ptx2_buffer
+
+    /\ handshake_state_m_disjoint_to_p2 hs p2
+    /\ handshake_state_m_disjoint_to_lbuffer hs ptx2_buffer
+    /\ B.loc_disjoint (plaintext2_union p2) (loc ptx2_buffer)
+  )
+  (ensures fun h0 _ h1 ->
+    let modified_locs = lbufferOpt_loc hs.prk3e2m |+| plaintext2_union p2 in
+
+    modifies modified_locs h0 h1
+    /\ is_valid_handshake_state_m h1 hs
+    /\ is_valid_plaintext2 h1 p2
+    /\ lbufferOpt_is_Some h1 hs.prk3e2m
+  )
+  = ST.push_frame();
+  (**) let h0 = ST.get () in
+
+  // derive SALT3e2m
+  let salt3e2m = create (hash_size_t kcs) (u8 0) in
+  expand_salt #kcs SpecKS.info_label_salt3e2m hs.prk2e.value hs.th2.value salt3e2m;
+  (**) let h2 = ST.get () in
+
+  // derive PRK3e2m
+  extract_prk3e2m #kcs salt3e2m hs.k_auth_R hs.prk3e2m.value;
+  lbufferOpt_set_Some hs.prk3e2m; // set Some for prk3e2m
+  (**) let h3 = ST.get () in
+
+  // deserialize plaintext2
+  deserialize_ptx2 kcs ptx2_buffer p2;
+  (**) let h4 = ST.get () in
+  (**) assert(
+    let modified_locs = loc salt3e2m
+                        |+| lbufferOpt_loc hs.prk3e2m
+                        |+| plaintext2_union p2 in
+    modifies modified_locs h0 h4
+  );
+
+  ST.pop_frame();
+  (**) let h_final = ST.get () in
+  ()
+
+let initiator_process_msg2_decrypt_c2 kcs is hs msg2 ptx2
+  = (**) let h0 = ST.get () in
+  ST.push_frame();
+
+  // create a buffer containing un-deserialized plaintext2
+  let ptx2_buffer = create (plaintext2_size_t kcs) (u8 0) in
+  let res = decrypt_ciphertext2 #kcs msg2.c2 hs.th2.value hs.prk2e.value ptx2_buffer in
+  (**) let h1 = ST.get () in
+  let final_res = match res with
+    | TypeEdhoc.CUnsupportedAlgorithmOrInvalidConfig
+    | TypeEdhoc.CDecryptionFailure -> res
+    | TypeEdhoc.CSuccess -> (
+      (**) assert(modifies1 ptx2_buffer h0 h1);
+      initiator_process_msg2_decrypt_c2_set_up hs ptx2 ptx2_buffer;
+
+      initiator_process_msg2_decrypt_c2_uti #kcs hs is ptx2
+    ) in
+
+  ST.pop_frame();
+  (**) let h_final = ST.get () in
+  (**) assert(res == TypeEdhoc.CSuccess ==> (
+    modifies (lbufferOpt_loc hs.prk3e2m |+| plaintext2_union ptx2) h0 h_final
+  ));
+  final_res
+
+
+#pop-options
 
 (*----------------- Responder's side*)
 val responder_send_msg2_set_up:
