src/kemedhoc/Impl.KEMEDHOC.Core.Msg2.fst
@@ -38,6 +38,8 @@ let responder_send_msg2 kcs rs hs msg1 msg2
     /\ lbufferOpt_is_Some h_final hs.prk3e2m
   );
   (**) assume(
+    res <> TypeEdhoc.CUnsupportedAlgorithmOrInvalidConfig
+    ==> (
     let rs_init = party_state_m_eval h0 rs in
     let hs_init = handshake_state_m_eval h0 hs in
     let msg1_init = message1_eval h0 msg1 in
@@ -55,12 +57,41 @@ let responder_send_msg2 kcs rs hs msg1 msg2
         /\ Spec.hs_equal hs_s_final hs_s
         /\ SpecParser.message2_equal msg2_s_final m2_s
       )
-    
-    );
+    ));
     res
-
-#pop-options
 
 (*------------------ Initiator's side*)
 let initiator_process_msg2 kcs is hs msg2 p2
-  = TypeEdhoc.CSuccess
+  = (**) let h0 = ST.get () in
+  initiator_process_msg2_set_up kcs is hs msg2;
+  let res = initiator_process_msg2_decrypt_c2 kcs is hs msg2 p2 in
+
+  (**) let h_final = ST.get () in
+  (**) assert(
+    lbufferOpt_is_Some h_final hs.k_xy /\ lbufferOpt_is_Some h_final hs.k_auth_I
+    /\ lbufferOpt_is_Some h_final hs.th2 /\ lbufferOpt_is_Some h_final hs.prk2e
+    /\ (res == TypeEdhoc.CSuccess ==> lbufferOpt_is_Some h_final hs.prk3e2m)
+  );
+  (**) assume(
+    res <> TypeEdhoc.CUnsupportedAlgorithmOrInvalidConfig
+    ==> (
+      let rs_init = party_state_m_eval h0 is in
+      let hs_init = handshake_state_m_eval h0 hs in
+      let msg2_init = message2_eval h0 msg2 in
+
+      let res_s = Spec.initiator_process_msg2 kcs rs_init hs_init msg2_init in
+      let hs_s_final = handshake_state_m_eval h_final hs in
+
+      match res_s with
+        | Fail e -> error_to_c_response e == res
+        | Res (hs_s, p2_s) -> (
+          res == TypeEdhoc.CSuccess
+          /\ Spec.hs_equal hs_s_final hs_s
+          /\ SpecParser.plaintext2_equal (plaintext2_eval h_final p2) p2_s
+        )
+    )
+  );
+  res
+
+#pop-options
+
