src/kemedhoc/Impl.KEMEDHOC.Core.Utilities.fst
@@ -1,0 +1,84 @@
+module Impl.KEMEDHOC.Core.Utilities
+
+(*HACL related modules*)
+// open Lib.RawIntTypes
+open Lib.IntTypes
+// open Lib.Sequence
+open Lib.ByteBuffer
+// lbuffer type, an immutable buffer with
+// length tag, is from this module
+// let lbuffer (a:Type0) (len:size_t) = lbuffer_t MUT a len
+// `live` and `disjoint` are also from this module.
+// Basically, HACL `Lib.Buffer` is a wrapper of `LowStar.Buffer`
+// and related LowStar memory models.
+open Lib.Buffer
+
+open Impl.KEMEDHOC.Types
+
+(*LowStar related modules*)
+module B = LowStar.Buffer
+module ST = FStar.HyperStack.ST
+module HS = FStar.HyperStack
+module S = FStar.Seq
+module Seq = Lib.Sequence
+
+module SpecParser = Spec.KEMEDHOC.Parser
+module SpecCrypto = Spec.KEMEDHOC.CryptoPrimitives
+module TypeEdhoc = TypeHelper.EDHOC
+
+
+open Impl.KEMEDHOC.CryptoPrimitives
+open Impl.KEMEDHOC.Types
+open Impl.KEMEDHOC.Parser
+open Spec.KEMEDHOC.Base.Definitions
+
+
+open LowStar.BufferOps
+
+/// Check Credential
+val check_credential:
+  cred_A: id_cred_buffer
+  -> cred_B: id_cred_buffer
+  -> ST.Stack c_response
+  (requires fun h0 ->
+    live h0 cred_A /\ live h0 cred_B
+  )
+  (ensures fun h0 res h1 -> (res == TypeEdhoc.CSuccess \/ res == TypeEdhoc.CInvalidCredential)
+    /\ modifies0 h0 h1
+    /\ (match res with
+      | TypeEdhoc.CSuccess -> (
+        (Seq.equal (as_seq h0 cred_A) (as_seq h0 cred_B))
+      )
+      | TypeEdhoc.CInvalidCredential ->
+        ~(Seq.equal (as_seq h0 cred_A) (as_seq h0 cred_B))
+      | _ -> False
+    )
+  )
+
+let check_credential cred_A cred_B
+  = if (lbytes_eq cred_A cred_B) then TypeEdhoc.CSuccess
+  else TypeEdhoc.CInvalidCredential
+
+/// Check MAC
+val check_mac:
+  #kcs: supportedKemCipherSuite
+  -> mac_A: mac23_buff kcs
+  -> mac_B: mac23_buff kcs
+  -> ST.Stack c_response
+  (requires fun h0 ->
+    live h0 mac_A /\ live h0 mac_B
+  )
+  (ensures fun h0 res h1 ->
+    let res_s = Seq.equal (as_seq h0 mac_A) (as_seq h0 mac_B) in
+
+    modifies0 h0 h1
+    /\ (match res with
+      | TypeEdhoc.CSuccess -> res_s
+      | TypeEdhoc.CIntegrityCheckFailed -> ~res_s
+      | _ -> False
+    )
+  )
+
+let check_mac #kcs mac_A mac_B
+  = if (lbytes_eq mac_A mac_B) then TypeEdhoc.CSuccess
+  else TypeEdhoc.CIntegrityCheckFailed
